Manual/BuiltInTypes/String/FFI.lean
@@ -1,0 +1,43 @@
+import Verso.Genre.Manual
+
+import Manual.Meta
+open Manual.FFIDocType
+
+open Verso.Genre Manual
+
+set_option pp.rawOnError true
+
+
+#doc (Manual) "FFI" =>
+
+{docstring String.csize}
+
+:::ffi "lean_string_object" kind := type
+```
+typedef struct {
+    lean_object m_header;
+    /* byte length including '\0' terminator */
+    size_t      m_size;
+    size_t      m_capacity;
+    /* UTF8 length */
+    size_t      m_length;
+    char        m_data[0];
+} lean_string_object;
+```
+TODO xref to runtime representation above
+:::
+
+:::ffi "lean_is_string"
+````
+bool lean_is_string(lean_object * o)
+````
+
+Returns `true` if `o` is a string, or `false` otherwise.
+:::
+
+:::ffi "lean_to_string"
+````
+lean_string_object * lean_to_string(lean_object * o)
+````
+Performs a runtime check that `o` is indeed a string. If `o` is not a string, an assertion fails.
+:::
