Manual/BuiltInTypes/String/Literals.lean
@@ -1,0 +1,95 @@
+import Verso.Genre.Manual
+
+import Manual.Meta
+open Manual.FFIDocType
+
+open Verso.Genre Manual
+
+set_option pp.rawOnError true
+
+
+#doc (Manual) "Syntax" =>
+
+# Syntax
+
+Lean has two kinds of string literals: ordinary string literals and raw string literals.
+
+## String Literals
+
+String literals begin and end with a double-quote character `"`. {index subterm:="string"}[literal]
+Between these characters, they may contain any other character, including newlines, which are included literally (with the caveat that all newlines in a Lean source file are interpreted as `'\n'`, regardless of file encoding and platform).
+Special characters that cannot otherwise be written in string literals may be escaped with a backslash, so `"\"Quotes\""` is a string literal that begins and ends with double quotes.
+The following forms of escape sequences are accepted:
+
+: `\r`, `\n`, `\t`, `\\`, `\"`, `\'`
+
+  These escape sequences have the usual meaning, mapping to `CR`, `LF`, tab, backslash, double quote, and single quote, respectively.
+
+: `\xNN`
+
+  When `NN` is a sequence of two hexadecimal digits, this escape denotes the character whose Unicode codepoint is indicated by the two-digit hexadecimal code.
+
+: `\uNNNN`
+
+  When `NN` is a sequence of two hexadecimal digits, this escape denotes the character whose Unicode codepoint is indicated by the four-digit hexadecimal code.
+
+
+String literals may contain {deftech}[_gaps_].
+A gap is indicated by an escaped newline, with no intervening characters between the escaping backslash and the newline.
+In this case, the string denoted by the literal is missing the newline and all leading whitespace from the next line.
+String gaps may not precede lines that contain only whitespace.
+
+Here, `str1` and `str2` are the same string:
+```lean
+def str1 := "String with \
+             a gap"
+def str2 := "String with a gap"
+
+example : str1 = str2 := rfl
+```
+
+This example is rejected, because the line following the gap is empty:
+
+```
+def str3 := "String with \
+
+             a gap"
+```
+
+
+## Raw String Literals
+
+In {deftech}[raw string literals], {index subterm:="raw string"}[literal] there are no escape sequences or gaps, and each character denotes itself exactly.
+Raw string literals are preceded by `r`, followed by zero or more hash characters (`#`) and a double quote `"`.
+The string literal is completed at a double quote that is followed by _the same number_ of hash characters.
+For example, they can be used to avoid the need to double-escape certain characters:
+```lean
+example : r"\t" = "\\t" := rfl
+-- TODO get this message in CI and in the text
+#eval r"Write backslash in a string using '\\\\'"
+```
+
+Including hash marks allows the strings to contain unescaped quotes:
+
+```lean
+example : r#"This is "literally" quoted"# = "This is \"literally\" quoted" := rfl
+```
+
+Adding sufficiently many hash marks allows any raw literal to be written literally:
+
+```lean
+example : r##"This is r#"literally"# quoted"## = "This is r#\"literally\"# quoted" := rfl
+```
+
+
+## Interpolated Strings
+
+Preceding a string literal with `s!` causes it to be processed as an {deftech}[_interpolated string_], in which regions of the string surrounded by `{` and `}` characters are parsed and interpreted as Lean expressions.
+Interpolated strings are interpreted by appending the string that precedes the interpolation, the expression (with an added call to {name ToString.toString}`toString` surrounding it), and the string that follows the interpolation.
+
+For example:
+```lean
+example : s!"1 + 1 = {1 + 1}\n" = "1 + 1 = " ++ toString (1 + 1) ++ "\n" := rfl
+```
+
+Preceding a literal with `m!` causes the interpolation to result in an instance of {name Lean.MessageData}`MessageData`, the compiler's internal data structure for messages to be shown to users.
