Manual/BuiltInTypes/String/Logical.lean
@@ -1,0 +1,16 @@
+import Verso.Genre.Manual
+
+import Manual.Meta
+open Manual.FFIDocType
+
+open Verso.Genre Manual
+
+set_option pp.rawOnError true
+
+
+#doc (Manual) "Logical Model" =>
+
+{docstring String}
+
+The logical model of strings in Lean is a structure that contains a single field, which is a list of characters.
+This is convenient when specifying and proving properties of string-processing fuctions at a low level.
