Manual/Language.lean
@@ -1,0 +1,162 @@
+import Verso.Genre.Manual
+
+import Manual.Meta
+
+open Verso.Genre Manual
+
+set_option pp.rawOnError true
+
+set_option linter.unusedVariables false
+
+#doc (Manual) "The Lean Language" =>
+
+# Types
+
+## Functions
+
+
+## Propositions
+
+Propositions are meaningful statements that admit proof. {index}[proposition]
+Nonsensical statements are not propositions, but false statements are.
+All propositions are classified by `Prop`.
+
+Propositions have the following properties:
+
+: Definitional proof irrelevance
+
+  Any two proofs of the same proposition are completely interchangeable.
+
+: Run-time irrelevance
+
+  Propositions are erased from compiled code.
+
+: Impredicativity
+
+  Propositions may quantify over types from any universe whatsoever.
+
+: Restricted Elimination
+
+  With the exception of singletons, propositions cannot be eliminated into non-proposition types.
+
+
+## Universes
+
+Types are classified by _universes_. {index}[universe]
+Each universe has a {deftech (key:="universe level")}[_level_], {index subterm := "of universe"}[level] which is a natural number.
+The `Sort` operator constructs a universe from a given level. {index}[`Sort`]
+If the level of a universe is smaller than that of another, the universe itself is said to be smaller.
+With the exception of propositions (described later in this chapter), types in a given universe may only quantify over types in smaller universes.
+`Sort 0` is the type of propositions, while each `Sort (u + 1)` is a type that describes data.
+
+Every universe is an element of every strictly larger universe, so `Sort 5` includes `Sort 4`.
+This means that the following examples are accepted:
+```lean
+example : Sort 5 := Sort 4
+example : Sort 2 := Sort 1
+```
+
+On the other hand, `Sort 3` is not an element of `Sort 5`:
+```lean error := true name := sort3
+example : Sort 5 := Sort 3
+```
+
+TODO show output
+
+Similarly, because `Unit` is in `Sort 1`, it is not in `Sort 2`:
+```lean
+example : Sort 1 := Unit
+```
+```lean error := true
+example : Sort 2 := Unit
+```
+
+TODO show output
+
+Because propositions and data are used differently and are governed by different rules, the abbreviations `Type` and `Prop` are provided to make the distinction more convenient.  {index}[`Type`] {index}[`Prop`]
+`Type u` is an abbreviation for `Sort (u + 1)`, so `Type 0` is `Sort 1` and `Type 3` is `Sort 4`.
+`Type 0` can also be abbreviated `Type`, so `Unit : Type` and `Type : Type 1`.
+`Prop` is an abbreviation for `Sort 0`.
+
+### Predicativity
+
+Each universe contains dependent function types, which additionally represent universal quantification and implication.
+A function type's universe is determined by the universes of its argument and return types.
+The specific rules depend on whether the return type of the function is a proposition.
+
+Functions that return propositions (that is, where the result type of the function is some type in `Prop`) may have argument types in any universe whatsoever, and the function type itself is in `Prop`.
+In other words, propositions feature _impredicative_ {index}[impredicative]{index subterm := "impredicative"}[quantification] quantification, because propositions can themselves be statements about all propositions.
+For example, proof irrelevance can be written as a proposition that quantifies over all propositions:
+```lean
+example : Prop := ∀ (P : Prop) (p1 p2 : P), p1 = p2
+```
+
+For universes at {tech key:="universe level"}[level] `1` and higher (that is, the `Type u` hierarchy), quantification is {deftech}[_predicative_]. {index}[predicative]{index subterm := "predicative"}[quantification]
+For these universes, the universe of a function type is the greater of the argument and return types' universes.
+
+```lean
+example (α : Type 1) (β : Type 2) : Type 2 := α → β
+example (α : Type 2) (β : Type 1) : Type 2 := α → β
+```
+
+This example is not accepted, because `α`'s level is greater than `1`. In other words, the annotated universe is smaller than the function type's universe:
+```lean error := true
+example (α : Type 2) (β : Type 1) : Type 1 := α → β
+```
+This example is not accepted because the annotated universe is larger than the function type's universe:
+```lean error := true
+example (α : Type 2) (β : Type 1) : Type 3 := α → β
+```
+
+### Polymorphism
+
+Lean supports _universe polymorphism_, {index subterm:="universe"}[polymorphism] {index}[universe polymorphism] which means that constants defined in the Lean environment can take universe parameters.
+These parameters can then be instantiated with universe levels when the constant is used.
+Universe parameters are written in curly braces following a dot after a constant name.
+
+When fully explicit, the identity function takes a universe parameter `u`:
+```lean
+def identity.{u} {α : Sort u} (x : α) : α := x
+```
+
+TODO port signature macro from blog genre
+
+```lean
+#check id
+```
+
+This means that `id` can be applied to types in _any_ universe.
+Conceptually speaking, `id` is a schematic definition that defines a family of identity functions, one for each universe.
+
+#### Level Expressions
+
+Levels that occur in a definition are not restricted to just variables.
+More complex relationships between universes can be defined using level expressions.
+
+
+````
+Level ::= n                -- Concrete levels
+        | u, v             -- Variables
+        | Level + n        -- Addition of constants
+        | max Level Level  -- Least upper bound
+        | imax Level Level -- Impredicative LUB
+````
+
+Given an assignment of level variables to concrete numbers, evaluating these expressions follows the usual rules of arithmetic.
+The `imax` operation is defined as follows:
+
+$``\mathtt{imax}\ u\ v = \begin{cases}{cl}0 & \mathrm{when }v = 0\\\mathtt{max}\ u\ v&\mathrm{otherwise}\end{cases}``
+
+TODO examples
+
+#### Universe Variable Bindings
+
+TODO `universe` command, local universe vars, auto-implicits
+
+#### Unification
+
+TODO injectivity, (defaulting?)
+
+
+
+## Inductive Types
