lakefile.lean
@@ -8,6 +8,54 @@ package "verso-manual" where
 
 lean_lib Manual where
 
+def inputTextFile' (path : FilePath) : SpawnM (BuildJob FilePath) :=
+  Job.async do (path, ·) <$> computeTrace (TextFilePath.mk path)
+
+def figureDir : FilePath := "figures"
+def figureOutDir : FilePath := "static/figures"
+
+def ensureDir (dir : System.FilePath) : IO Unit := do
+  if !(← dir.pathExists) then
+    IO.FS.createDirAll dir
+  if !(← dir.isDir) then
+    throw (↑ s!"Not a directory: {dir}")
+
+
+target figures : Array FilePath := do
+  let files := (← figureDir.readDir).filterMap fun f =>
+    match f.path.extension with
+    | some "tex" => some f.path
+    | _ => none
+  let files := files.qsort (toString · < toString ·)
+  IO.println files
+  let srcs ← BuildJob.collectArray (← liftM <| files.mapM inputTextFile')
+  let traceFile := figureDir.join "lake.trace"
+  liftM <| srcs.bindSync fun srcInfo depTrace => do
+    buildUnlessUpToDate traceFile depTrace traceFile do
+      for src in srcInfo do
+        let some f := src.fileStem
+          | continue
+        proc { cmd := "lualatex", args := #[f], cwd := some figureDir} (quiet := true)
+        proc { cmd := "lualatex", args := #[f], cwd := some figureDir} (quiet := true)
+        proc { cmd := "lualatex", args := #[f], cwd := some figureDir} (quiet := true)
+        proc { cmd := "lualatex", args := #[f], cwd := some figureDir} (quiet := true)
+        proc { cmd := "pdftocairo", args := #["-svg", s!"{f}.pdf", s!"{f}.svg"], cwd := some figureDir} (quiet := true)
+
+        ensureDir "static"
+        ensureDir figureOutDir
+        for fmt in ["pdf", "svg"] do
+          IO.println s!"Format: {fmt}"
+          let built := s!"{f}.{fmt}"
+          IO.FS.withFile (figureDir.join built) .read fun h =>
+            IO.FS.withFile (figureOutDir.join built) .write fun h' => do
+              let mut buf ← h.read 1024
+              while !buf.isEmpty do
+                h'.write buf
+                buf ← h.read 1024
+
+    pure (srcInfo, depTrace)
+
 @[default_target]
 lean_exe "generate-manual" where
+  extraDepTargets := #[`figures]
   root := `Main
